Nats.thy
@@ -181,7 +181,7 @@ proof (rule ccontr, auto)
     also have "... = (\<f> \<circ>\<^sub>c \<beta>\<^bsub>\<Omega>\<^esub>) \<circ>\<^sub>c u \<circ>\<^sub>c n"
       using assms u_type by (typecheck_cfuncs, simp add:  comp_associative2 u_square)
     also have "... = \<f>"
-      using assms u_type by (typecheck_cfuncs, metis cfunc_type_def comp_associative id_right_unit2 id_type terminal_func_comp terminal_func_unique)
+      using assms u_type by (etcs_assocr,typecheck_cfuncs, simp add: id_right_unit2 terminal_func_comp_elem)
     then show ?thesis using calculation by auto
   qed
   then show False
@@ -243,10 +243,10 @@ lemma zUs_surj:
 lemma nonzero_is_succ_aux:
   assumes "x \<in>\<^sub>c (one \<Coprod> \<nat>\<^sub>c)"
   shows "(x = (left_coproj one \<nat>\<^sub>c) \<circ>\<^sub>c id one) \<or>
-         (\<exists>n. (n \<in>\<^sub>c \<nat>\<^sub>c) \<and> (x = (right_coproj one \<nat>\<^sub>c) \<circ>\<^sub>c n ))"
-proof(auto)
+         (\<exists>n. (n \<in>\<^sub>c \<nat>\<^sub>c) \<and> (x = (right_coproj one \<nat>\<^sub>c) \<circ>\<^sub>c n))"
+proof auto
   assume "\<forall> n. n \<in>\<^sub>c  \<nat>\<^sub>c  \<longrightarrow>  x \<noteq> right_coproj one \<nat>\<^sub>c \<circ>\<^sub>c n"
-  then show "x = left_coproj one \<nat>\<^sub>c  \<circ>\<^sub>c  id one"
+  then show "x = left_coproj one \<nat>\<^sub>c \<circ>\<^sub>c id one"
     using assms coprojs_jointly_surj one_unique_element by (typecheck_cfuncs, blast)
 qed
 
@@ -536,21 +536,21 @@ next
     using assms cfunc_cross_prod_comp_cfunc_prod id_left_unit2 by (typecheck_cfuncs, force)
   also have "... = (eval_func (U\<^bsup>U\<^esup>) (U\<^bsup>U\<^esup>)) \<circ>\<^sub>c \<langle>f \<circ>\<^sub>c z, (ITER_curried U \<circ>\<^sub>c successor) \<circ>\<^sub>c (n  \<circ>\<^sub>c z)\<rangle>"
     using assms by(typecheck_cfuncs, metis comp_associative2)
-  also have "... = (eval_func (U\<^bsup>U\<^esup>) (U\<^bsup>U\<^esup>)) \<circ>\<^sub>c \<langle>f \<circ>\<^sub>c z, ((meta_comp U U U \<circ>\<^sub>c (id (U\<^bsup>U\<^esup>) \<times>\<^sub>f eval_func (U\<^bsup>U\<^esup>) (U\<^bsup>U\<^esup>)) \<circ>\<^sub>c (associate_right (U\<^bsup>U\<^esup>) (U\<^bsup>U\<^esup>) ((U\<^bsup>U\<^esup>)\<^bsup>U\<^bsup>U\<^esup>\<^esup>)) \<circ>\<^sub>c (diagonal(U\<^bsup>U\<^esup>)\<times>\<^sub>f id ((U\<^bsup>U\<^esup>)\<^bsup>U\<^bsup>U\<^esup>\<^esup>)))\<^sup>\<sharp>    \<circ>\<^sub>c ITER_curried U) \<circ>\<^sub>c (n  \<circ>\<^sub>c z)\<rangle>"
+  also have "... = (eval_func (U\<^bsup>U\<^esup>) (U\<^bsup>U\<^esup>)) \<circ>\<^sub>c \<langle>f \<circ>\<^sub>c z, ((meta_comp U U U \<circ>\<^sub>c (id (U\<^bsup>U\<^esup>) \<times>\<^sub>f eval_func (U\<^bsup>U\<^esup>) (U\<^bsup>U\<^esup>)) \<circ>\<^sub>c (associate_right (U\<^bsup>U\<^esup>) (U\<^bsup>U\<^esup>) ((U\<^bsup>U\<^esup>)\<^bsup>U\<^bsup>U\<^esup>\<^esup>)) \<circ>\<^sub>c (diagonal(U\<^bsup>U\<^esup>)\<times>\<^sub>f id ((U\<^bsup>U\<^esup>)\<^bsup>U\<^bsup>U\<^esup>\<^esup>)))\<^sup>\<sharp> \<circ>\<^sub>c ITER_curried U) \<circ>\<^sub>c (n  \<circ>\<^sub>c z)\<rangle>"
     using assms ITER_curried_successor by presburger
-  also have "... = (eval_func (U\<^bsup>U\<^esup>) (U\<^bsup>U\<^esup>)) \<circ>\<^sub>c (id (U\<^bsup>U\<^esup>) \<times>\<^sub>f ((meta_comp U U U \<circ>\<^sub>c (id (U\<^bsup>U\<^esup>) \<times>\<^sub>f eval_func (U\<^bsup>U\<^esup>) (U\<^bsup>U\<^esup>)) \<circ>\<^sub>c (associate_right (U\<^bsup>U\<^esup>) (U\<^bsup>U\<^esup>) ((U\<^bsup>U\<^esup>)\<^bsup>U\<^bsup>U\<^esup>\<^esup>)) \<circ>\<^sub>c (diagonal(U\<^bsup>U\<^esup>)\<times>\<^sub>f id ((U\<^bsup>U\<^esup>)\<^bsup>U\<^bsup>U\<^esup>\<^esup>)))\<^sup>\<sharp>    \<circ>\<^sub>c ITER_curried U) \<circ>\<^sub>c (n  \<circ>\<^sub>c z))\<circ>\<^sub>c \<langle>f \<circ>\<^sub>c z, id one\<rangle>"
+  also have "... = (eval_func (U\<^bsup>U\<^esup>) (U\<^bsup>U\<^esup>)) \<circ>\<^sub>c (id (U\<^bsup>U\<^esup>) \<times>\<^sub>f ((meta_comp U U U \<circ>\<^sub>c (id (U\<^bsup>U\<^esup>) \<times>\<^sub>f eval_func (U\<^bsup>U\<^esup>) (U\<^bsup>U\<^esup>)) \<circ>\<^sub>c (associate_right (U\<^bsup>U\<^esup>) (U\<^bsup>U\<^esup>) ((U\<^bsup>U\<^esup>)\<^bsup>U\<^bsup>U\<^esup>\<^esup>)) \<circ>\<^sub>c (diagonal(U\<^bsup>U\<^esup>)\<times>\<^sub>f id ((U\<^bsup>U\<^esup>)\<^bsup>U\<^bsup>U\<^esup>\<^esup>)))\<^sup>\<sharp> \<circ>\<^sub>c ITER_curried U) \<circ>\<^sub>c (n  \<circ>\<^sub>c z))\<circ>\<^sub>c \<langle>f \<circ>\<^sub>c z, id one\<rangle>"
     using assms by (typecheck_cfuncs, simp add: cfunc_cross_prod_comp_cfunc_prod id_left_unit2 id_right_unit2)
-  also have "... = (eval_func (U\<^bsup>U\<^esup>) (U\<^bsup>U\<^esup>)) \<circ>\<^sub>c (id (U\<^bsup>U\<^esup>) \<times>\<^sub>f ((meta_comp U U U \<circ>\<^sub>c (id (U\<^bsup>U\<^esup>) \<times>\<^sub>f eval_func (U\<^bsup>U\<^esup>) (U\<^bsup>U\<^esup>)) \<circ>\<^sub>c (associate_right (U\<^bsup>U\<^esup>) (U\<^bsup>U\<^esup>) ((U\<^bsup>U\<^esup>)\<^bsup>U\<^bsup>U\<^esup>\<^esup>)) \<circ>\<^sub>c (diagonal(U\<^bsup>U\<^esup>)\<times>\<^sub>f id ((U\<^bsup>U\<^esup>)\<^bsup>U\<^bsup>U\<^esup>\<^esup>)))\<^sup>\<sharp>     ))\<circ>\<^sub>c \<langle>f \<circ>\<^sub>c z, ITER_curried U \<circ>\<^sub>c (n  \<circ>\<^sub>c z)\<rangle>"
+  also have "... = (eval_func (U\<^bsup>U\<^esup>) (U\<^bsup>U\<^esup>)) \<circ>\<^sub>c (id (U\<^bsup>U\<^esup>) \<times>\<^sub>f ((meta_comp U U U \<circ>\<^sub>c (id (U\<^bsup>U\<^esup>) \<times>\<^sub>f eval_func (U\<^bsup>U\<^esup>) (U\<^bsup>U\<^esup>)) \<circ>\<^sub>c (associate_right (U\<^bsup>U\<^esup>) (U\<^bsup>U\<^esup>) ((U\<^bsup>U\<^esup>)\<^bsup>U\<^bsup>U\<^esup>\<^esup>)) \<circ>\<^sub>c (diagonal(U\<^bsup>U\<^esup>)\<times>\<^sub>f id ((U\<^bsup>U\<^esup>)\<^bsup>U\<^bsup>U\<^esup>\<^esup>)))\<^sup>\<sharp> ))\<circ>\<^sub>c \<langle>f \<circ>\<^sub>c z, ITER_curried U \<circ>\<^sub>c (n  \<circ>\<^sub>c z)\<rangle>"
     using assms by (typecheck_cfuncs, smt (z3) cfunc_cross_prod_comp_cfunc_prod comp_associative2 id_right_unit2)
-  also have "... = (meta_comp U U U \<circ>\<^sub>c (id (U\<^bsup>U\<^esup>) \<times>\<^sub>f eval_func (U\<^bsup>U\<^esup>) (U\<^bsup>U\<^esup>)) \<circ>\<^sub>c (associate_right (U\<^bsup>U\<^esup>) (U\<^bsup>U\<^esup>) ((U\<^bsup>U\<^esup>)\<^bsup>U\<^bsup>U\<^esup>\<^esup>)) \<circ>\<^sub>c (diagonal(U\<^bsup>U\<^esup>)\<times>\<^sub>f id ((U\<^bsup>U\<^esup>)\<^bsup>U\<^bsup>U\<^esup>\<^esup>)     ))\<circ>\<^sub>c \<langle>f \<circ>\<^sub>c z, ITER_curried U \<circ>\<^sub>c (n  \<circ>\<^sub>c z)\<rangle>"
+  also have "... = (meta_comp U U U \<circ>\<^sub>c (id (U\<^bsup>U\<^esup>) \<times>\<^sub>f eval_func (U\<^bsup>U\<^esup>) (U\<^bsup>U\<^esup>)) \<circ>\<^sub>c (associate_right (U\<^bsup>U\<^esup>) (U\<^bsup>U\<^esup>) ((U\<^bsup>U\<^esup>)\<^bsup>U\<^bsup>U\<^esup>\<^esup>)) \<circ>\<^sub>c (diagonal(U\<^bsup>U\<^esup>)\<times>\<^sub>f id ((U\<^bsup>U\<^esup>)\<^bsup>U\<^bsup>U\<^esup>\<^esup>)))\<circ>\<^sub>c \<langle>f \<circ>\<^sub>c z, ITER_curried U \<circ>\<^sub>c (n  \<circ>\<^sub>c z)\<rangle>"
     using assms by (typecheck_cfuncs, metis cfunc_type_def comp_associative transpose_func_def)
-  also have "... = (meta_comp U U U \<circ>\<^sub>c (id (U\<^bsup>U\<^esup>) \<times>\<^sub>f eval_func (U\<^bsup>U\<^esup>) (U\<^bsup>U\<^esup>)) \<circ>\<^sub>c (associate_right (U\<^bsup>U\<^esup>) (U\<^bsup>U\<^esup>) ((U\<^bsup>U\<^esup>)\<^bsup>U\<^bsup>U\<^esup>\<^esup>)) )\<circ>\<^sub>c \<langle>\<langle>f \<circ>\<^sub>c z,f \<circ>\<^sub>c z\<rangle>, ITER_curried U \<circ>\<^sub>c (n  \<circ>\<^sub>c z)\<rangle>"
+  also have "... = (meta_comp U U U \<circ>\<^sub>c (id (U\<^bsup>U\<^esup>) \<times>\<^sub>f eval_func (U\<^bsup>U\<^esup>) (U\<^bsup>U\<^esup>)) \<circ>\<^sub>c (associate_right (U\<^bsup>U\<^esup>) (U\<^bsup>U\<^esup>) ((U\<^bsup>U\<^esup>)\<^bsup>U\<^bsup>U\<^esup>\<^esup>)))\<circ>\<^sub>c \<langle>\<langle>f \<circ>\<^sub>c z,f \<circ>\<^sub>c z\<rangle>, ITER_curried U \<circ>\<^sub>c (n  \<circ>\<^sub>c z)\<rangle>"
     using assms by (etcs_assocr, typecheck_cfuncs, smt (z3) cfunc_cross_prod_comp_cfunc_prod diag_on_elements id_left_unit2)
-  also have "... = meta_comp U U U \<circ>\<^sub>c (id (U\<^bsup>U\<^esup>) \<times>\<^sub>f eval_func (U\<^bsup>U\<^esup>) (U\<^bsup>U\<^esup>)) \<circ>\<^sub>c   \<langle>f \<circ>\<^sub>c z, \<langle>f \<circ>\<^sub>c z, ITER_curried U \<circ>\<^sub>c (n  \<circ>\<^sub>c z)\<rangle>\<rangle>"
+  also have "... = meta_comp U U U \<circ>\<^sub>c (id (U\<^bsup>U\<^esup>) \<times>\<^sub>f eval_func (U\<^bsup>U\<^esup>) (U\<^bsup>U\<^esup>)) \<circ>\<^sub>c \<langle>f \<circ>\<^sub>c z, \<langle>f \<circ>\<^sub>c z, ITER_curried U \<circ>\<^sub>c (n  \<circ>\<^sub>c z)\<rangle>\<rangle>"
     using assms by (typecheck_cfuncs, smt (z3) associate_right_ap comp_associative2)
   also have "... = meta_comp U U U \<circ>\<^sub>c \<langle>f \<circ>\<^sub>c z, eval_func (U\<^bsup>U\<^esup>) (U\<^bsup>U\<^esup>) \<circ>\<^sub>c \<langle>f \<circ>\<^sub>c z, ITER_curried U \<circ>\<^sub>c (n  \<circ>\<^sub>c z)\<rangle>\<rangle>"
     using assms by (typecheck_cfuncs, smt (z3) cfunc_cross_prod_comp_cfunc_prod id_left_unit2)
-  also have "... = meta_comp U U U \<circ>\<^sub>c \<langle>f \<circ>\<^sub>c z, eval_func (U\<^bsup>U\<^esup>) (U\<^bsup>U\<^esup>) \<circ>\<^sub>c (id(U\<^bsup>U\<^esup>) \<times>\<^sub>f ITER_curried U )\<circ>\<^sub>c \<langle>f \<circ>\<^sub>c z,  (n  \<circ>\<^sub>c z)\<rangle>     \<rangle>"
+  also have "... = meta_comp U U U \<circ>\<^sub>c \<langle>f \<circ>\<^sub>c z, eval_func (U\<^bsup>U\<^esup>) (U\<^bsup>U\<^esup>) \<circ>\<^sub>c (id(U\<^bsup>U\<^esup>) \<times>\<^sub>f ITER_curried U)\<circ>\<^sub>c \<langle>f \<circ>\<^sub>c z, n \<circ>\<^sub>c z\<rangle>\<rangle>"
     using assms by (typecheck_cfuncs, smt (z3) cfunc_cross_prod_comp_cfunc_prod id_left_unit2)
   also have "... = meta_comp U U U \<circ>\<^sub>c \<langle>f \<circ>\<^sub>c z, ITER U \<circ>\<^sub>c \<langle>f \<circ>\<^sub>c z, n \<circ>\<^sub>c z\<rangle>\<rangle>"
     using assms by (typecheck_cfuncs, smt (z3) ITER_def comp_associative2 inv_transpose_func_def3)
@@ -566,14 +566,14 @@ qed
 
 lemma ITER_one:
  assumes "f \<in>\<^sub>c (U\<^bsup>U\<^esup>)"
- shows "ITER U \<circ>\<^sub>c \<langle>f, successor \<circ>\<^sub>c zero\<rangle> = f \<box> ( metafunc (id U))"
+ shows "ITER U \<circ>\<^sub>c \<langle>f, successor \<circ>\<^sub>c zero\<rangle> = f \<box> (metafunc (id U))"
   using ITER_succ ITER_zero' assms zero_type by presburger
 
 definition iter_comp :: "cfunc \<Rightarrow> cfunc \<Rightarrow> cfunc" ("_\<^bsup>\<circ>_\<^esup>"[55,0]55) where
   "iter_comp g n  \<equiv> cnufatem (ITER (domain g) \<circ>\<^sub>c \<langle>metafunc g,n\<rangle>)"
 
 lemma iter_comp_def2: 
-  "g\<^bsup>\<circ>n\<^esup>  \<equiv> cnufatem (ITER (domain g) \<circ>\<^sub>c \<langle>metafunc g,n\<rangle>)"
+  "g\<^bsup>\<circ>n\<^esup>  \<equiv> cnufatem(ITER (domain g) \<circ>\<^sub>c \<langle>metafunc g,n\<rangle>)"
   by (simp add: iter_comp_def)
 
 lemma iter_comp_type[type_rule]:
@@ -581,7 +581,7 @@ lemma iter_comp_type[type_rule]:
   assumes "n \<in>\<^sub>c \<nat>\<^sub>c"
   shows "g\<^bsup>\<circ>n\<^esup>: X \<rightarrow> X"
   unfolding iter_comp_def2
-  by (smt (verit, ccfv_SIG) ITER_type assms(1) assms(2) cfunc_type_def cnufatem_type comp_type metafunc_type right_param_on_el right_param_type) 
+  by (smt (verit, ccfv_SIG) ITER_type assms cfunc_type_def cnufatem_type comp_type metafunc_type right_param_on_el right_param_type) 
 
 lemma iter_comp_def3: 
   assumes "g : X \<rightarrow> X"
@@ -642,7 +642,7 @@ lemma eval_lemma_for_ITER:
   using assms by (typecheck_cfuncs, metis eval_lemma iter_comp_def3 metafunc_cnufatem)
 
 lemma n_accessible_by_succ_iter_aux:
-   "eval_func \<nat>\<^sub>c \<nat>\<^sub>c \<circ>\<^sub>c \<langle>zero \<circ>\<^sub>c \<beta>\<^bsub>\<nat>\<^sub>c\<^esub>,  ITER \<nat>\<^sub>c \<circ>\<^sub>c \<langle>(metafunc successor) \<circ>\<^sub>c \<beta>\<^bsub>\<nat>\<^sub>c\<^esub> ,id \<nat>\<^sub>c  \<rangle>\<rangle> = id \<nat>\<^sub>c"
+   "eval_func \<nat>\<^sub>c \<nat>\<^sub>c \<circ>\<^sub>c \<langle>zero \<circ>\<^sub>c \<beta>\<^bsub>\<nat>\<^sub>c\<^esub>,  ITER \<nat>\<^sub>c \<circ>\<^sub>c \<langle>(metafunc successor) \<circ>\<^sub>c \<beta>\<^bsub>\<nat>\<^sub>c\<^esub> ,id \<nat>\<^sub>c\<rangle>\<rangle> = id \<nat>\<^sub>c"
 proof(rule natural_number_object_func_unique[where X="\<nat>\<^sub>c", where f = successor])
   show "eval_func \<nat>\<^sub>c \<nat>\<^sub>c \<circ>\<^sub>c \<langle>zero \<circ>\<^sub>c \<beta>\<^bsub>\<nat>\<^sub>c\<^esub>,ITER \<nat>\<^sub>c \<circ>\<^sub>c \<langle>metafunc successor \<circ>\<^sub>c \<beta>\<^bsub>\<nat>\<^sub>c\<^esub>,id\<^sub>c \<nat>\<^sub>c\<rangle>\<rangle> : \<nat>\<^sub>c \<rightarrow> \<nat>\<^sub>c"
     by typecheck_cfuncs
@@ -652,9 +652,9 @@ proof(rule natural_number_object_func_unique[where X="\<nat>\<^sub>c", where f =
     by typecheck_cfuncs
 next
   have "(eval_func \<nat>\<^sub>c \<nat>\<^sub>c \<circ>\<^sub>c \<langle>zero \<circ>\<^sub>c \<beta>\<^bsub>\<nat>\<^sub>c\<^esub>,ITER \<nat>\<^sub>c \<circ>\<^sub>c \<langle>metafunc successor \<circ>\<^sub>c \<beta>\<^bsub>\<nat>\<^sub>c\<^esub>,id\<^sub>c \<nat>\<^sub>c\<rangle>\<rangle>) \<circ>\<^sub>c zero =
-         eval_func \<nat>\<^sub>c \<nat>\<^sub>c \<circ>\<^sub>c \<langle>zero \<circ>\<^sub>c \<beta>\<^bsub>\<nat>\<^sub>c\<^esub> \<circ>\<^sub>c zero,ITER \<nat>\<^sub>c \<circ>\<^sub>c \<langle>metafunc successor \<circ>\<^sub>c \<beta>\<^bsub>\<nat>\<^sub>c\<^esub> \<circ>\<^sub>c zero,id\<^sub>c \<nat>\<^sub>c \<circ>\<^sub>c zero\<rangle> \<rangle>"
+         eval_func \<nat>\<^sub>c \<nat>\<^sub>c \<circ>\<^sub>c \<langle>zero \<circ>\<^sub>c \<beta>\<^bsub>\<nat>\<^sub>c\<^esub> \<circ>\<^sub>c zero,ITER \<nat>\<^sub>c \<circ>\<^sub>c \<langle>metafunc successor \<circ>\<^sub>c \<beta>\<^bsub>\<nat>\<^sub>c\<^esub> \<circ>\<^sub>c zero,id\<^sub>c \<nat>\<^sub>c \<circ>\<^sub>c zero\<rangle>\<rangle>"
     by (typecheck_cfuncs, smt (z3) cfunc_prod_comp comp_associative2)
-  also have "... =  eval_func \<nat>\<^sub>c \<nat>\<^sub>c \<circ>\<^sub>c \<langle>zero,ITER \<nat>\<^sub>c \<circ>\<^sub>c \<langle>metafunc successor,zero\<rangle> \<rangle>"
+  also have "... =  eval_func \<nat>\<^sub>c \<nat>\<^sub>c \<circ>\<^sub>c \<langle>zero,ITER \<nat>\<^sub>c \<circ>\<^sub>c \<langle>metafunc successor,zero\<rangle>\<rangle>"
     by (typecheck_cfuncs, simp add: id_left_unit2 id_right_unit2 terminal_func_comp_elem)
   also have "... =  eval_func \<nat>\<^sub>c \<nat>\<^sub>c \<circ>\<^sub>c \<langle>zero,metafunc (id \<nat>\<^sub>c) \<rangle>"
     by (typecheck_cfuncs, simp add: ITER_zero')
@@ -673,7 +673,7 @@ next
     fix m
     assume m_type[type_rule]: "m \<in>\<^sub>c \<nat>\<^sub>c"
     have "(successor \<circ>\<^sub>c eval_func \<nat>\<^sub>c \<nat>\<^sub>c \<circ>\<^sub>c \<langle>zero \<circ>\<^sub>c \<beta>\<^bsub>\<nat>\<^sub>c\<^esub>,ITER \<nat>\<^sub>c \<circ>\<^sub>c \<langle>metafunc successor \<circ>\<^sub>c \<beta>\<^bsub>\<nat>\<^sub>c\<^esub>,id\<^sub>c \<nat>\<^sub>c\<rangle>\<rangle>) \<circ>\<^sub>c m = 
-         successor \<circ>\<^sub>c eval_func \<nat>\<^sub>c \<nat>\<^sub>c \<circ>\<^sub>c \<langle>zero \<circ>\<^sub>c \<beta>\<^bsub>\<nat>\<^sub>c\<^esub> \<circ>\<^sub>c m,ITER \<nat>\<^sub>c \<circ>\<^sub>c \<langle>metafunc successor \<circ>\<^sub>c \<beta>\<^bsub>\<nat>\<^sub>c\<^esub> \<circ>\<^sub>c m,id\<^sub>c \<nat>\<^sub>c \<circ>\<^sub>c m\<rangle>\<rangle> "
+         successor \<circ>\<^sub>c eval_func \<nat>\<^sub>c \<nat>\<^sub>c \<circ>\<^sub>c \<langle>zero \<circ>\<^sub>c \<beta>\<^bsub>\<nat>\<^sub>c\<^esub> \<circ>\<^sub>c m,ITER \<nat>\<^sub>c \<circ>\<^sub>c \<langle>metafunc successor \<circ>\<^sub>c \<beta>\<^bsub>\<nat>\<^sub>c\<^esub> \<circ>\<^sub>c m,id\<^sub>c \<nat>\<^sub>c \<circ>\<^sub>c m\<rangle>\<rangle>"
       by (typecheck_cfuncs, smt (z3) cfunc_prod_comp comp_associative2)
     also have "... = successor \<circ>\<^sub>c eval_func \<nat>\<^sub>c \<nat>\<^sub>c \<circ>\<^sub>c \<langle>zero ,ITER \<nat>\<^sub>c \<circ>\<^sub>c \<langle>metafunc successor ,m\<rangle>\<rangle>"
       by (typecheck_cfuncs, simp add: id_left_unit2 id_right_unit2 terminal_func_comp_elem)
@@ -681,9 +681,9 @@ next
       by (typecheck_cfuncs, simp add: eval_lemma_for_ITER)
     also have "... = (successor\<^bsup>\<circ>successor \<circ>\<^sub>c m\<^esup>) \<circ>\<^sub>c zero"
       by (typecheck_cfuncs, simp add: comp_associative2 succ_iters)
-    also have "... = eval_func \<nat>\<^sub>c \<nat>\<^sub>c \<circ>\<^sub>c \<langle>zero ,ITER \<nat>\<^sub>c \<circ>\<^sub>c \<langle>metafunc successor ,successor \<circ>\<^sub>c m\<rangle> \<rangle>"
+    also have "... = eval_func \<nat>\<^sub>c \<nat>\<^sub>c \<circ>\<^sub>c \<langle>zero ,ITER \<nat>\<^sub>c \<circ>\<^sub>c \<langle>metafunc successor ,successor \<circ>\<^sub>c m\<rangle>\<rangle>"
       by (typecheck_cfuncs, simp add: eval_lemma_for_ITER)
-    also have "... = eval_func \<nat>\<^sub>c \<nat>\<^sub>c \<circ>\<^sub>c \<langle>zero \<circ>\<^sub>c \<beta>\<^bsub>\<nat>\<^sub>c\<^esub> \<circ>\<^sub>c (successor \<circ>\<^sub>c m),ITER \<nat>\<^sub>c \<circ>\<^sub>c \<langle>metafunc successor \<circ>\<^sub>c \<beta>\<^bsub>\<nat>\<^sub>c\<^esub>\<circ>\<^sub>c (successor \<circ>\<^sub>c m),id\<^sub>c \<nat>\<^sub>c \<circ>\<^sub>c (successor \<circ>\<^sub>c m)\<rangle> \<rangle>"
+    also have "... = eval_func \<nat>\<^sub>c \<nat>\<^sub>c \<circ>\<^sub>c \<langle>zero \<circ>\<^sub>c \<beta>\<^bsub>\<nat>\<^sub>c\<^esub> \<circ>\<^sub>c (successor \<circ>\<^sub>c m),ITER \<nat>\<^sub>c \<circ>\<^sub>c \<langle>metafunc successor \<circ>\<^sub>c \<beta>\<^bsub>\<nat>\<^sub>c\<^esub>\<circ>\<^sub>c (successor \<circ>\<^sub>c m),id\<^sub>c \<nat>\<^sub>c \<circ>\<^sub>c (successor \<circ>\<^sub>c m)\<rangle>\<rangle>"
       by (typecheck_cfuncs,simp add: id_left_unit2 id_right_unit2 terminal_func_comp_elem)
     also have "... = ((eval_func \<nat>\<^sub>c \<nat>\<^sub>c \<circ>\<^sub>c \<langle>zero \<circ>\<^sub>c \<beta>\<^bsub>\<nat>\<^sub>c\<^esub>,ITER \<nat>\<^sub>c \<circ>\<^sub>c \<langle>metafunc successor \<circ>\<^sub>c \<beta>\<^bsub>\<nat>\<^sub>c\<^esub>,id\<^sub>c \<nat>\<^sub>c\<rangle>\<rangle>) \<circ>\<^sub>c successor) \<circ>\<^sub>c m"
       by (typecheck_cfuncs, smt (z3) cfunc_prod_comp comp_associative2)
@@ -701,9 +701,9 @@ lemma n_accessible_by_succ_iter:
 proof - 
   have "n = eval_func \<nat>\<^sub>c \<nat>\<^sub>c \<circ>\<^sub>c \<langle>zero \<circ>\<^sub>c \<beta>\<^bsub>\<nat>\<^sub>c\<^esub>, ITER \<nat>\<^sub>c \<circ>\<^sub>c \<langle>metafunc successor \<circ>\<^sub>c \<beta>\<^bsub>\<nat>\<^sub>c\<^esub>, id \<nat>\<^sub>c\<rangle>\<rangle> \<circ>\<^sub>c n"
     using assms by (typecheck_cfuncs, simp add: comp_associative2 id_left_unit2 n_accessible_by_succ_iter_aux)
-  also have "... = eval_func \<nat>\<^sub>c \<nat>\<^sub>c \<circ>\<^sub>c \<langle>zero \<circ>\<^sub>c \<beta>\<^bsub>\<nat>\<^sub>c\<^esub> \<circ>\<^sub>c n , ITER \<nat>\<^sub>c \<circ>\<^sub>c \<langle>metafunc successor \<circ>\<^sub>c \<beta>\<^bsub>\<nat>\<^sub>c\<^esub> \<circ>\<^sub>c n, id \<nat>\<^sub>c \<circ>\<^sub>c n\<rangle>\<rangle> "
+  also have "... = eval_func \<nat>\<^sub>c \<nat>\<^sub>c \<circ>\<^sub>c \<langle>zero \<circ>\<^sub>c \<beta>\<^bsub>\<nat>\<^sub>c\<^esub> \<circ>\<^sub>c n , ITER \<nat>\<^sub>c \<circ>\<^sub>c \<langle>metafunc successor \<circ>\<^sub>c \<beta>\<^bsub>\<nat>\<^sub>c\<^esub> \<circ>\<^sub>c n, id \<nat>\<^sub>c \<circ>\<^sub>c n\<rangle>\<rangle>"
     using assms by (typecheck_cfuncs, smt (z3) cfunc_prod_comp comp_associative2)
-  also have "... = eval_func \<nat>\<^sub>c \<nat>\<^sub>c \<circ>\<^sub>c \<langle>zero,  ITER \<nat>\<^sub>c \<circ>\<^sub>c \<langle>metafunc successor, n\<rangle>\<rangle> "
+  also have "... = eval_func \<nat>\<^sub>c \<nat>\<^sub>c \<circ>\<^sub>c \<langle>zero,  ITER \<nat>\<^sub>c \<circ>\<^sub>c \<langle>metafunc successor, n\<rangle>\<rangle>"
     using assms by (typecheck_cfuncs, simp add: id_left_unit2 id_right_unit2 terminal_func_comp_elem)
   also have "... = (successor\<^bsup>\<circ>n\<^esup>) \<circ>\<^sub>c zero"
     using assms by (typecheck_cfuncs, metis eval_lemma iter_comp_def3 metafunc_cnufatem)
